Blblblblb

RSA_games.ec
@@ -39,14 +39,18 @@ prime (s_q sk).
 op pkey_eq pk1 pk2 = (p_n pk1 = p_n pk2) /\ (p_e pk1 = p_e pk2).
 op skey_eq sk1 sk2 = (s_d sk1 = s_d sk2) /\ (s_p sk1 = s_p sk2) /\ (s_q sk1 = s_q sk2).
 
+const SK: skey.
+const PK: pkey.
+axiom valid_global : support keypairs (PK, SK).
+
 (* An adverseray trying to factor an rsa modulus n*)
 module type RSA_factoring_adv = {
   proc factorize(pk: pkey): int * int
 }.
 
 module RSA_factoring_game(Adv: RSA_factoring_adv) = {
-  var pk: pkey
-  var sk: skey
+  (*var pk: pkey
+  var sk: skey*)
 
   proc main() = {
     var p': int;
@@ -54,9 +58,9 @@ module RSA_factoring_game(Adv: RSA_factoring_adv) = {
 
     (*(pk, sk) <$ keypairs;*)
 
-    (p', q') <@ Adv.factorize(pk);
+    (p', q') <@ Adv.factorize(PK);
 
-    return ((p'*q') = p_n pk) && 1 < p' && p' < q' && q' < p_n pk;
+    return ((p'*q') = p_n PK) && 1 < p' && p' < q' && q' < p_n PK;
   }
 }.
 
@@ -65,16 +69,16 @@ module type RSA_GOP_adv = {
 }.
 
 module RSA_GOP(Adv: RSA_GOP_adv) = {
-  var pk: pkey
-  var sk: skey
+  (*var pk: pkey
+  var sk: skey*)
 
   proc main() = {
     var z: int;
 
     (*(pk, sk) <$ keypairs;*)
-    z <@ Adv.compute_GO(pk);
+    z <@ Adv.compute_GO(PK);
 
-    return z = (s_p sk - 1)*(s_q sk - 1);
+    return z = (s_p SK - 1)*(s_q SK - 1);
   }
 }.
 
@@ -95,6 +99,16 @@ declare module A <: RSA_factoring_adv.
     assume.
   *)
 
+lemma simple_red : equiv[RSA_factoring_game(A).main ~ RSA_GOP(B(A)).main : true ==> res{1} => res{2}].
+proof.
+proc.
+inline *.
+simplify.
+auto.
+apply valid_global.
+trivial.
+smt.
+
 (* Reduction from factoring to GOP, when using B(A) as an adversary.
   The precondition is that we consider the same parameters in both games, and that those are valid*)
 lemma red : equiv[RSA_factoring_game(A).main ~ RSA_GOP(B(A)).main :
@@ -103,7 +117,20 @@ lemma red : equiv[RSA_factoring_game(A).main ~ RSA_GOP(B(A)).main :
       /\ (support keypairs (RSA_factoring_game.pk{1}, RSA_factoring_game.sk{1}))
       /\ (support keypairs (RSA_GOP.pk{2}, RSA_GOP.sk{2}))
       ==> res{1} => res{2}].
+proof.
+progress.
+proc.
+inline *.
+auto.
+move=> ->.
+smt.
 
+smt.
+apply valid_keypairs.
+reflexivity.
+rewrite pkey_eq.
+inline pkey_eq.
+smt.
 
 lemma reduction &m: Pr[RSA_factoring_game(A).main() @ &m: res] <= Pr[RSA_GOP(B(A)).main() @ &m: res].
     proof.
